Mica/Verifier/Expressions.lean
@@ -200,6 +200,7 @@ mutual
   def compile (reg : Verifier.Registry) (Θ : TinyML.TypeEnv) (Δ_spec : Signature) (S : SpecMap) (B : Bindings) (Γ : TinyML.TyCtx) : Expr → VerifM (Term .value)
     | .const (.int n)  => pure (.unop .ofInt  (.const (.i n)))
     | .const (.bool b) => pure (.unop .ofBool (.const (.b b)))
+    | .const (.char c) => pure (.unop .ofChar (.const (.char c)))
     | .const (.string s) => pure (.unop .ofString (.const (.str s)))
     | .const (.float b) => pure (.unop .ofFloat (.const (.fp b)))
     | .const .unit     => pure (Term.const .unit)
@@ -674,6 +675,22 @@ theorem compileConst_correct (reg : Verifier.Registry) (c : TinyML.Const) :
     · iexact Howns
     · isplitl []
       · exact TinyML.ValHasType.bool_intro Θ b
+      · iexact HR
+  | char c =>
+    simp only [compile] at heval
+    simp only [Expr.runtime, Runtime.Val.ofConst, Runtime.Expr.subst_val]
+    obtain heval := VerifM.eval_ret heval
+    simp only [Expr.ty, Const.ty] at hpost
+    refine SpatialContext.wp_val ?_
+    istart
+    iintro ⟨Howns, _HS, _Hts, HR⟩
+    iapply (hpost (.char c) ρ st _ heval
+      (by simp [Term.wfIn, Const.wfIn, UnOp.wfIn])
+      (by simp [Term.eval, UnOp.eval, Const.denote]))
+    isplitl [Howns]
+    · iexact Howns
+    · isplitl []
+      · exact TinyML.ValHasType.char_intro Θ c
       · iexact HR
   | string s =>
     simp only [compile] at heval
